Better rule for function application with wps. How to test compilation?

rupicola/refinements/EquivRel.fsti
@@ -1,7 +1,9 @@
 module EquivRel
 
-open FStar.Tactics
 open FStar.Classical.Sugar
+open FStar.Tactics
+open FStar.Calc
+
 open FStar.List.Tot
 
 open STLC
@@ -52,7 +54,7 @@ let rec (∋) (t:typsr) (p:get_Type t * closed_exp) : Tot Type0 (decreases %[get
     FStar.Monotonic.Pure.elim_pure_wp_monotonicity_forall ();
     match e with
     | ELam e' ->
-      (forall (v:value) (fs_v:s1).
+      (forall (v:value) fs_v.
         (| t1, s1, r1 |) ∋ (fs_v, v) /\ as_requires (wp fs_v) ==>  (** Interesting that we do not need to quantify over post-conditions because of monotonicity **)
          (| t2, s2, r2 |) ⦂ (fs_f fs_v, subst_beta v e'))
     | _ -> False
@@ -108,7 +110,9 @@ type gpre (g:env) =
   fs_env g -> Type0
 
 type fs_oexp (#g:env) (pre:gpre g) (a:Type) =
-  s:(fs_env g) -> Pure a (pre s) (fun _ -> True)
+  fs_s:(fs_env g) -> Pure a (pre fs_s) (fun _ -> True)
+               (**  ^^^^ here probably we have the monad we compile.
+                    This will give us the initial state/history over which to state the pre-condition**)
 
 (** Cross Language Binary Logical Relation between F* and STLC expressions
      for __open terms__. **)
@@ -203,24 +207,58 @@ let equiv_lam
 let mk_pre_app #g (pre:gpre g) (#t1 #t2:Type) (wp:t1 -> pure_wp t2) (fs_e:fs_oexp pre t1) : gpre g =
   fun fs_s -> pre fs_s /\ as_requires (wp (fs_e fs_s))
 
+unfold
+let helper_fapp wp (f:(x:'a -> PURE 'b (wp x))) (x:'a) : Pure 'b (as_requires (wp x)) (fun _ -> True) =
+  FStar.Monotonic.Pure.elim_pure_wp_monotonicity_forall ();
+  f x
+
+let get_rel' = get_rel
+
+let lem_super_lemma (t2:typsr) :
+  Lemma (t2._2 == get_Type t2)
+         by (norm [delta_only [`%get_Type];iota])= ()
+
+let eliminate_value_arrow (t1 t2:typsr) wp fs_e1 e11 fs_e2 (e2:value) :
+  Lemma
+    (requires (is_closed (ELam e11) /\ as_requires (wp fs_e2) /\ is_closed e2 /\
+               mk_arrow_wp t1 t2 wp ∋ (fs_e1, ELam e11) /\ t1 ∋ (fs_e2, e2)))
+    (ensures  (t2 ⦂ (helper_fapp wp fs_e1 fs_e2, subst_beta e2 e11))) =
+    calc (<==>) {
+      mk_arrow_wp t1 t2 wp ∋ (fs_e1, ELam e11);
+      <==> { _ by (
+               norm [delta_once [`%mk_arrow_wp; `%op_u8715;`%get_rel;`%Mkdtuple3?._3;`%snd;`%Mktuple2?._2;`%fst;`%Mktuple2?._1];zeta;iota];
+               norm [delta_only [`%get_rel';`%helper_fapp];iota]
+          )}
+      (forall (v:value) (fs_v:t1._2). (| t1._1, t1._2, get_rel' t1 |) ∋ (fs_v, v) /\ as_requires #t2._2 (wp fs_v)  ==>
+                 (| t2._1, t2._2, get_rel' t2 |) ⦂ (helper_fapp #t1._2 #t2._2 wp fs_e1 fs_v, subst_beta v e11));
+      <==> { _ by (norm [delta_only [`%get_rel'];iota]) }
+      (forall (v:value) fs_v. t1 ∋ (fs_v, v) /\ as_requires #t2._2 (wp fs_v)  ==>
+                 (| t2._1, t2._2, get_rel t2 |) ⦂ (helper_fapp #t1._2 #t2._2 wp fs_e1 fs_v, subst_beta v e11));
+      <==> { _ by (l_to_r [`lem_super_lemma]) }
+      (forall (v:value) fs_v. t1 ∋ (fs_v, v) /\ as_requires (wp fs_v)  ==>
+                 (| t2._1, t2._2, get_rel t2 |) ⦂ (helper_fapp wp fs_e1 fs_v, subst_beta v e11));
+    }
+
 let equiv_app
   g (pre:gpre g)
   (t1:typsr) (t2:typsr) (wp:get_Type t1 -> pure_wp (get_Type t2))
   (e1:exp)
   (fs_e1:fs_oexp pre (get_Type (mk_arrow_wp t1 t2 wp)))
   (e2:exp)
-  (fs_e2:fs_oexp pre (get_Type t1)) : Lemma
-  (requires fs_e1 `equiv _ pre` e1 /\ fs_e2 `equiv _ pre` e2)
-  (ensures
-    equiv #g t2 (mk_pre_app pre wp fs_e2)
-      (fun fs_s -> FStar.Monotonic.Pure.elim_pure_wp_monotonicity_forall (); (fs_e1 fs_s) (fs_e2 fs_s))
-      (EApp e1 e2)) =
+  (fs_e2:fs_oexp pre (get_Type t1))
+  (l:squash (forall fs_s. pre fs_s ==>  as_requires (wp (fs_e2 fs_s))))
+  : Lemma
+    (requires fs_e1 `equiv _ pre` e1 /\ fs_e2 `equiv _ pre` e2)
+    (ensures
+      equiv #g t2 pre //(mk_pre_app pre wp fs_e2)
+        (fun fs_s -> FStar.Monotonic.Pure.elim_pure_wp_monotonicity_forall (); (fs_e1 fs_s) (fs_e2 fs_s))
+        (EApp e1 e2)) =
   FStar.Monotonic.Pure.elim_pure_wp_monotonicity_forall ();
   lem_fv_in_env_app g e1 e2;
-  let pre' : gpre g = (mk_pre_app pre wp fs_e2) in
-  let fs_e : fs_oexp pre' (get_Type t2) = fun fs_s -> (fs_e1 fs_s) (fs_e2 fs_s) in
-  introduce forall b (s:gsub g b) fs_s. s ∽ fs_s /\ pre' fs_s ==> t2 ⦂ (fs_e fs_s, gsubst s (EApp e1 e2)) with begin
-    introduce s ∽ fs_s /\ pre' fs_s ==>  _ with _. begin
+ // let pre' : gpre g = (mk_pre_app pre wp fs_e2) in
+  let fs_e : fs_oexp pre (get_Type t2) = fun fs_s -> (fs_e1 fs_s) (fs_e2 fs_s) in
+  introduce forall b (s:gsub g b) fs_s. s ∽ fs_s /\ pre fs_s ==> t2 ⦂ (fs_e fs_s, gsubst s (EApp e1 e2)) with begin
+    introduce s ∽ fs_s /\ pre fs_s ==>  _ with _. begin
       let fs_e1' : (x:get_Type t1 -> PURE (get_Type t2) (wp x)) = fs_e1 fs_s in
       let fs_e2' = fs_e2 fs_s in
       assert (as_requires (wp fs_e2'));
@@ -229,19 +267,12 @@ let equiv_app
           let steps_e_e' : squash (steps (EApp (gsubst s e1) (gsubst s e2)) e') = () in
           FStar.Squash.map_squash #_ #(squash (t2 ∋ (fs_e fs_s, e'))) steps_e_e' (fun steps_e_e' ->
             let (e11, e2') = destruct_steps_eapp (gsubst s e1) (gsubst s e2) e' steps_e_e' in
-            assert (mk_arrow_wp t1 t2 wp ∋ (fs_e1', ELam e11));
-            assert (t1 ∋ (fs_e2', e2'));
-            (**
-            let fs_res = fs_e1' fs_e2' in
-            eliminate True /\ True
-            returns t2 ⦂ (fs_res, subst_beta e2' e11) with _ _. begin
-              assert (forall (v:value) (fs_v:get_Type t1). t1 ∋ (fs_v, v) /\ as_requires (wp fs_v)  ==>
-                      t2 ⦂ (fs_e1' fs_v, subst_beta v e11))
-              //with e2' fs_e2'
+            eliminate mk_arrow_wp t1 t2 wp ∋ (fs_e1', ELam e11) /\ t1 ∋ (fs_e2', e2')
+            returns t2 ⦂ (helper_fapp wp fs_e1' fs_e2', subst_beta e2' e11) with h1 _. begin
+              eliminate_value_arrow t1 t2 wp fs_e1' e11 fs_e2' e2'
             end;
-            assert (t2 ⦂ (fs_e, subst_beta e2' e11));
-            assert (t2 ∋ (fs_e, e'))**)
-            admit ()
+            assert (t2 ⦂ (fs_e fs_s, subst_beta e2' e11));
+            assert (t2 ∋ (fs_e fs_s, e'))
           )
         end
       end
